theories/lang_oadt/admissible.v
@@ -9,41 +9,48 @@ From oadt Require Import lang_oadt.equivalence.
 Import syntax.notations.
 Import semantics.notations.
 Import typing.notations.
+Import equivalence.notations.
 
 Implicit Types (b : bool) (x X y Y : atom) (L : aset) (T : lexpr).
 
 #[local]
 Coercion EFVar : atom >-> expr.
 
+Section admissible.
+
+Context (Σ : gctx).
+Context (Hwf : gctx_wf Σ).
+
+#[local]
+Set Default Proof Using "Hwf".
+
 (** * Admissible step introduction rules *)
 
 (** * Renaming lemmas *)
 
-Lemma typing_kinding_rename_ Σ x y T :
-  gctx_wf Σ ->
+Lemma typing_kinding_rename_ x y T :
   (forall Γ' e l τ,
-      Σ; Γ' ⊢ e :{l} τ ->
+      Γ' ⊢ e :{l} τ ->
       forall Γ,
         Γ' = <[x:=T]>Γ ->
         x ∉ fv T ∪ dom aset Γ ->
         y ∉ {[x]} ∪ fv e ∪ fv T ∪ dom aset Γ ->
-        Σ; (<[y:=T]>({x↦y} <$> Γ)) ⊢ {x↦y}e :{l} {x↦y}τ) /\
+        <[y:=T]>({x↦y} <$> Γ) ⊢ {x↦y}e :{l} {x↦y}τ) /\
   (forall Γ' τ κ,
-      Σ; Γ' ⊢ τ :: κ ->
+      Γ' ⊢ τ :: κ ->
       forall Γ,
         Γ' = <[x:=T]>Γ ->
         x ∉ fv T ∪ dom aset Γ ->
         y ∉ {[x]} ∪ fv τ ∪ fv T ∪ dom aset Γ ->
-        Σ; (<[y:=T]>({x↦y} <$> Γ)) ⊢ {x↦y}τ :: κ).
+        <[y:=T]>({x↦y} <$> Γ) ⊢ {x↦y}τ :: κ).
 Proof.
-  intros Hwf.
   apply typing_kinding_mutind; intros; subst; simpl in *;
     (* First we normalize the typing and kinding judgments so they are ready
     for applying typing and kinding rules to. *)
     rewrite ?subst_open_distr by constructor;
     rewrite ?subst_ite_distr;
     try lazymatch goal with
-        | |- _; _ ⊢ [inj@_< ?ω > _] : {_↦_}?ω =>
+        | |- _ ⊢ [inj@_< ?ω > _] : {_↦_}?ω =>
           rewrite subst_fresh by shelve
         | |- context [decide (_ = _)] =>
           case_decide; subst
@@ -75,8 +82,8 @@ Proof.
       Otherwise some existential variables may have undesirable
       instantiation. *)
       lazymatch goal with
-      | |- _; ?Γ ⊢ _ : _ => go Γ
-      | |- _; ?Γ ⊢ _ :: _ => go Γ
+      | |- ?Γ ⊢ _ : _ => go Γ
+      | |- ?Γ ⊢ _ :: _ => go Γ
       | _ => idtac
       end;
         (* Try to solve other side conditions. *)
@@ -88,7 +95,7 @@ Proof.
                  shelve
                | |- <[_:=_]>(<[_:=_]>_) = <[_:=_]>(<[_:=_]>_) =>
                  apply insert_commute
-               | |- _ ⊢ _ ≡ _ =>
+               | |- _ ≡ _ =>
                  apply pared_equiv_rename
                | |- <[?y:=_]>_ !! ?y = Some _ =>
                  simplify_map_eq
@@ -113,12 +120,11 @@ Proof.
 Qed.
 
 (** We also allow [x=y]. *)
-Lemma typing_rename_ Σ Γ e l τ T x y :
-  gctx_wf Σ ->
-  Σ; (<[x:=T]>Γ) ⊢ e :{l} τ ->
+Lemma typing_rename_ Γ e l τ T x y :
+  <[x:=T]>Γ ⊢ e :{l} τ ->
   x ∉ fv T ∪ dom aset Γ ->
   y ∉ fv e ∪ fv T ∪ dom aset Γ ->
-  Σ; (<[y:=T]>({x↦y} <$> Γ)) ⊢ {x↦y}e :{l} {x↦y}τ.
+  <[y:=T]>({x↦y} <$> Γ) ⊢ {x↦y}e :{l} {x↦y}τ.
 Proof.
   intros.
   destruct (decide (y = x)); subst.
@@ -126,12 +132,11 @@ Proof.
   - qauto use: typing_kinding_rename_ solve: fast_set_solver!!.
 Qed.
 
-Lemma kinding_rename_ Σ Γ τ T κ x y :
-  gctx_wf Σ ->
-  Σ; (<[x:=T]>Γ) ⊢ τ :: κ ->
+Lemma kinding_rename_ Γ τ T κ x y :
+  <[x:=T]>Γ ⊢ τ :: κ ->
   x ∉ fv T ∪ dom aset Γ ->
   y ∉ fv τ ∪ fv T ∪ dom aset Γ ->
-  Σ; (<[y:=T]>({x↦y} <$> Γ)) ⊢ {x↦y}τ :: κ.
+  <[y:=T]>({x↦y} <$> Γ) ⊢ {x↦y}τ :: κ.
 Proof.
   intros.
   destruct (decide (y = x)); subst.
@@ -141,19 +146,19 @@ Qed.
 
 (** The actual renaming lemmas. The side conditions are slightly different than
 the general version. *)
-Lemma typing_rename_alt Σ Γ e l s τ T x y :
-  gctx_wf Σ ->
-  Σ; (<[x:=T]>Γ) ⊢ e^x :{l} τ^({y↦x}s) ->
+Lemma typing_rename_alt Γ e l s τ T x y :
+  <[x:=T]>Γ ⊢ e^x :{l} τ^({y↦x}s) ->
   x ∉ fv T ∪ fv e ∪ fv τ ∪ fv s ∪ dom aset Γ ∪ tctx_fv Γ ->
   y ∉ fv T ∪ fv e ∪ dom aset Γ ->
-  Σ; (<[y:=T]>Γ) ⊢ e^y :{l} τ^s.
+  <[y:=T]>Γ ⊢ e^y :{l} τ^s.
 Proof.
   intros.
   destruct (decide (y = x)); subst.
   - srewrite subst_id; eauto.
   - rewrite <- (subst_tctx_fresh Γ x y) by fast_set_solver!!.
     rewrite (subst_intro e y x) by fast_set_solver!!.
-    apply_eq typing_rename_; eauto.
+    relax_typing_type.
+    apply typing_rename_; eauto.
     fast_set_solver!!.
     simpl_fv. fast_set_solver!!.
     rewrite subst_open_distr by constructor.
@@ -163,12 +168,11 @@ Proof.
     eauto.
 Qed.
 
-Lemma typing_rename Σ Γ e l τ T x y :
-  gctx_wf Σ ->
-  Σ; (<[x:=T]>Γ) ⊢ e^x :{l} τ^x ->
+Lemma typing_rename Γ e l τ T x y :
+  <[x:=T]>Γ ⊢ e^x :{l} τ^x ->
   x ∉ fv T ∪ fv e ∪ fv τ ∪ dom aset Γ ∪ tctx_fv Γ ->
   y ∉ fv T ∪ fv e ∪ dom aset Γ ->
-  Σ; (<[y:=T]>Γ) ⊢ e^y :{l} τ^y.
+  <[y:=T]>Γ ⊢ e^y :{l} τ^y.
 Proof.
   intros.
   destruct (decide (y = x)); subst; eauto.
@@ -177,12 +181,11 @@ Proof.
   fast_set_solver!!.
 Qed.
 
-Lemma kinding_rename Σ Γ τ κ T x y :
-  gctx_wf Σ ->
-  Σ; (<[x:=T]>Γ) ⊢ τ^x :: κ ->
+Lemma kinding_rename Γ τ κ T x y :
+  <[x:=T]>Γ ⊢ τ^x :: κ ->
   x ∉ fv T ∪ fv τ ∪ dom aset Γ ∪ tctx_fv Γ ->
   y ∉ fv T ∪ fv τ ∪ dom aset Γ ->
-  Σ; (<[y:=T]>Γ) ⊢ τ^y :: κ.
+  <[y:=T]>Γ ⊢ τ^y :: κ.
 Proof.
   intros.
   destruct (decide (y = x)); subst; eauto.
@@ -193,142 +196,126 @@ Proof.
   simpl_fv. fast_set_solver!!.
 Qed.
 
-Lemma typing_rename_lc Σ Γ e l τ T x y :
-  gctx_wf Σ ->
-  Σ; (<[x:=T]>Γ) ⊢ e^x :{l} τ ->
+Lemma typing_rename_lc Γ e l τ T x y :
+  <[x:=T]>Γ ⊢ e^x :{l} τ ->
   x ∉ fv T ∪ fv e ∪ fv τ ∪ dom aset Γ ∪ tctx_fv Γ ->
   y ∉ fv T ∪ fv e ∪ dom aset Γ ->
-  Σ; (<[y:=T]>Γ) ⊢ e^y :{l} τ.
+  <[y:=T]>Γ ⊢ e^y :{l} τ.
 Proof.
-  intros Hwf H. intros.
+  intros H. intros.
   erewrite <- (open_lc_intro τ y) by eauto using typing_type_lc.
   erewrite <- (open_lc_intro τ x) in H by eauto using typing_type_lc.
   eapply typing_rename; eauto.
 Qed.
 
 (** * Admissible typing and kinding introduction rules *)
-Section typing_kinding_intro.
 
-  Context {Σ : gctx} (Hwf : gctx_wf Σ).
+Ltac typing_intro_solver :=
+  intros; econstructor; eauto; simpl_cofin?;
+  lazymatch goal with
+  | |- _ ⊢ _ : _^(fvar _) => eapply typing_rename
+  | |- _ ⊢ _ : _^_ => eapply typing_rename_alt; try relax_typing_type
+  | |- _ ⊢ _ : _ => eapply typing_rename_lc
+  | |- _ ⊢ _ :: _ => eapply kinding_rename
+  end; eauto;
+    try match goal with
+        | |- _ ∉ _ => try fast_set_solver!!; simpl_fv; fast_set_solver!!
+        end.
 
-  #[local]
-  Set Default Proof Using "Hwf".
+Lemma TAbs_intro Γ e l1 l2 τ1 τ2 κ x :
+  <[x:=(l2, τ2)]>Γ ⊢ e^x :{l1} τ1^x ->
+  Γ ⊢ τ2 :: κ ->
+  x ∉ fv e ∪ fv τ1 ∪ dom aset Γ ∪ tctx_fv Γ ->
+  Γ ⊢ \:{l2}τ2 => e :{l1} (Π:{l2}τ2, τ1).
+Proof.
+  typing_intro_solver.
+Qed.
 
-  Notation "Γ '⊢' e ':{' l '}' τ" := (Σ; Γ ⊢ e :{l} τ)
-                                       (at level 40,
-                                        e custom oadt at level 99,
-                                        τ custom oadt at level 99).
-  Notation "Γ '⊢' τ '::' κ" := (Σ; Γ ⊢ τ :: κ)
-                                 (at level 40,
-                                  τ custom oadt at level 99,
-                                  κ custom oadt at level 99).
+Lemma TLet_intro Γ l1 l2 l e1 e2 τ1 τ2 x :
+  Γ ⊢ e1 :{l1} τ1 ->
+  <[x:=(l1, τ1)]>Γ ⊢ e2^x :{l2} τ2^x ->
+  l = l1 ⊔ l2 ->
+  x ∉ fv e2 ∪ fv τ2 ∪ dom aset Γ ∪ tctx_fv Γ ->
+  Γ ⊢ let e1 in e2 :{l} τ2^e1.
+Proof.
+  typing_intro_solver.
+Qed.
 
-  Ltac typing_intro_solver :=
-    intros; econstructor; eauto; simpl_cofin?;
-    lazymatch goal with
-    | |- _ ⊢ _ :{_} _^(fvar _) => eapply typing_rename
-    | |- _ ⊢ _ :{_} _^_ => eapply typing_rename_alt; try relax_typing_type
-    | |- _ ⊢ _ :{_} _ => eapply typing_rename_lc
-    | |- _ ⊢ _ :: _ => eapply kinding_rename
-    end; eauto;
-      try match goal with
-          | |- _ ∉ _ => try fast_set_solver!!; simpl_fv; fast_set_solver!!
-          end.
+Lemma TCase_intro Γ l1 l2 l e0 e1 e2 τ1 τ2 τ κ x :
+  Γ ⊢ e0 :{⊥} τ1 + τ2 ->
+  <[x:=(⊥, τ1)]>Γ ⊢ e1^x :{l1} τ^(inl<τ1 + τ2> x) ->
+  <[x:=(⊥, τ2)]>Γ ⊢ e2^x :{l2} τ^(inr<τ1 + τ2> x) ->
+  Γ ⊢ τ^e0 :: κ ->
+  l = l1 ⊔ l2 ->
+  x ∉ fv e1 ∪ fv e2 ∪ fv τ ∪ dom aset Γ ∪ tctx_fv Γ ->
+  Γ ⊢ case e0 of e1 | e2 :{l} τ^e0.
+Proof.
+  typing_intro_solver.
 
-  Lemma TAbs_intro Γ e l1 l2 τ1 τ2 κ x :
-    <[x:=(l2, τ2)]>Γ ⊢ e^x :{l1} τ1^x ->
-    Γ ⊢ τ2 :: κ ->
-    x ∉ fv e ∪ fv τ1 ∪ dom aset Γ ∪ tctx_fv Γ ->
-    Γ ⊢ \:{l2}τ2 => e :{l1} (Π:{l2}τ2, τ1).
-  Proof.
-    typing_intro_solver.
-  Qed.
+  all : simpl; rewrite decide_True by eauto;
+    rewrite !subst_fresh by fast_set_solver!!; eauto.
+Qed.
 
-  Lemma TLet_intro Γ l1 l2 l e1 e2 τ1 τ2 x :
-    Γ ⊢ e1 :{l1} τ1 ->
-    <[x:=(l1, τ1)]>Γ ⊢ e2^x :{l2} τ2^x ->
-    l = l1 ⊔ l2 ->
-    x ∉ fv e2 ∪ fv τ2 ∪ dom aset Γ ∪ tctx_fv Γ ->
-    Γ ⊢ let e1 in e2 :{l} τ2^e1.
-  Proof.
-    typing_intro_solver.
-  Qed.
+Lemma TCaseNoDep_intro Γ l0 l1 l2 l e0 e1 e2 τ1 τ2 τ κ x :
+  Γ ⊢ e0 :{l0} τ1 + τ2 ->
+  <[x:=(l0, τ1)]>Γ ⊢ e1^x :{l1} τ ->
+  <[x:=(l0, τ2)]>Γ ⊢ e2^x :{l2} τ ->
+  Γ ⊢ τ :: κ ->
+  l = l0 ⊔ l1 ⊔ l2 ->
+  x ∉ fv e1 ∪ fv e2 ∪ fv τ ∪ dom aset Γ ∪ tctx_fv Γ ->
+  Γ ⊢ case e0 of e1 | e2 :{l} τ.
+Proof.
+  typing_intro_solver.
+Qed.
 
-  Lemma TCase_intro Γ l1 l2 l e0 e1 e2 τ1 τ2 τ κ x :
-    Γ ⊢ e0 :{⊥} τ1 + τ2 ->
-    <[x:=(⊥, τ1)]>Γ ⊢ e1^x :{l1} τ^(inl<τ1 + τ2> x) ->
-    <[x:=(⊥, τ2)]>Γ ⊢ e2^x :{l2} τ^(inr<τ1 + τ2> x) ->
-    Γ ⊢ τ^e0 :: κ ->
-    l = l1 ⊔ l2 ->
-    x ∉ fv e1 ∪ fv e2 ∪ fv τ ∪ dom aset Γ ∪ tctx_fv Γ ->
-    Γ ⊢ case e0 of e1 | e2 :{l} τ^e0.
-  Proof.
-    typing_intro_solver.
+Lemma TOCase_intro Γ l1 l2 e0 e1 e2 τ1 τ2 τ κ x :
+  Γ ⊢ e0 :{⊥} τ1 ~+ τ2 ->
+  <[x:=(⊥, τ1)]>Γ ⊢ e1^x :{l1} τ ->
+  <[x:=(⊥, τ2)]>Γ ⊢ e2^x :{l2} τ ->
+  Γ ⊢ τ :: κ ->
+  x ∉ fv e1 ∪ fv e2 ∪ dom aset Γ ∪ tctx_fv Γ ->
+  Γ ⊢ ~case e0 of e1 | e2 :{⊤} τ.
+Proof.
+  typing_intro_solver.
+Qed.
 
-    all : simpl; rewrite decide_True by eauto;
-      rewrite !subst_fresh by fast_set_solver!!; eauto.
-  Qed.
+Lemma KPi_intro Γ l τ1 τ2 κ1 κ2 x :
+  <[x:=(l, τ1)]>Γ ⊢ τ2^x :: κ2 ->
+  Γ ⊢ τ1 :: κ1 ->
+  x ∉ fv τ2 ∪ dom aset Γ ∪ tctx_fv Γ ->
+  Γ ⊢ (Π:{l}τ1, τ2) :: *@M.
+Proof.
+  typing_intro_solver.
+Qed.
 
-  Lemma TCaseNoDep_intro Γ l0 l1 l2 l e0 e1 e2 τ1 τ2 τ κ x :
-    Γ ⊢ e0 :{l0} τ1 + τ2 ->
-    <[x:=(l0, τ1)]>Γ ⊢ e1^x :{l1} τ ->
-    <[x:=(l0, τ2)]>Γ ⊢ e2^x :{l2} τ ->
-    Γ ⊢ τ :: κ ->
-    l = l0 ⊔ l1 ⊔ l2 ->
-    x ∉ fv e1 ∪ fv e2 ∪ fv τ ∪ dom aset Γ ∪ tctx_fv Γ ->
-    Γ ⊢ case e0 of e1 | e2 :{l} τ.
-  Proof.
-    typing_intro_solver.
-  Qed.
+Lemma KCase_intro Γ e0 τ1 τ2 τ1' τ2' x :
+  Γ ⊢ e0 :{⊥} τ1' + τ2' ->
+  <[x:=(⊥, τ1')]>Γ ⊢ τ1^x :: *@O ->
+  <[x:=(⊥, τ2')]>Γ ⊢ τ2^x :: *@O ->
+  x ∉ fv τ1 ∪ fv τ2 ∪ dom aset Γ ∪ tctx_fv Γ ->
+  Γ ⊢ case e0 of τ1 | τ2 :: *@O.
+Proof.
+  typing_intro_solver.
+Qed.
 
-  Lemma TOCase_intro Γ l1 l2 e0 e1 e2 τ1 τ2 τ κ x :
-    Γ ⊢ e0 :{⊥} τ1 ~+ τ2 ->
-    <[x:=(⊥, τ1)]>Γ ⊢ e1^x :{l1} τ ->
-    <[x:=(⊥, τ2)]>Γ ⊢ e2^x :{l2} τ ->
-    Γ ⊢ τ :: κ ->
-    x ∉ fv e1 ∪ fv e2 ∪ dom aset Γ ∪ tctx_fv Γ ->
-    Γ ⊢ ~case e0 of e1 | e2 :{⊤} τ.
-  Proof.
-    typing_intro_solver.
-  Qed.
+Lemma KLet_intro Γ e τ τ' x :
+  Γ ⊢ e :{⊥} τ' ->
+  <[x:=(⊥, τ')]>Γ ⊢ τ^x :: *@O ->
+  x ∉ fv τ ∪ dom aset Γ ∪ tctx_fv Γ ->
+  Γ ⊢ let e in τ :: *@O.
+Proof.
+  typing_intro_solver.
+Qed.
 
-  Lemma KPi_intro Γ l τ1 τ2 κ1 κ2 x :
-    <[x:=(l, τ1)]>Γ ⊢ τ2^x :: κ2 ->
-    Γ ⊢ τ1 :: κ1 ->
-    x ∉ fv τ2 ∪ dom aset Γ ∪ tctx_fv Γ ->
-    Γ ⊢ (Π:{l}τ1, τ2) :: *@M.
-  Proof.
-    typing_intro_solver.
-  Qed.
+Lemma KProd_intro Γ τ1 τ2 κ1 κ2 :
+  Γ ⊢ τ1 :: κ1 ->
+  Γ ⊢ τ2 :: κ2 ->
+  Γ ⊢ τ1 * τ2 :: (κ1 ⊔ κ2).
+Proof.
+  eauto using kinding, join_ub_l, join_ub_r.
+Qed.
 
-  Lemma KCase_intro Γ e0 τ1 τ2 τ1' τ2' x :
-    Γ ⊢ e0 :{⊥} τ1' + τ2' ->
-    <[x:=(⊥, τ1')]>Γ ⊢ τ1^x :: *@O ->
-    <[x:=(⊥, τ2')]>Γ ⊢ τ2^x :: *@O ->
-    x ∉ fv τ1 ∪ fv τ2 ∪ dom aset Γ ∪ tctx_fv Γ ->
-    Γ ⊢ case e0 of τ1 | τ2 :: *@O.
-  Proof.
-    typing_intro_solver.
-  Qed.
-
-  Lemma KLet_intro Γ e τ τ' x :
-    Γ ⊢ e :{⊥} τ' ->
-    <[x:=(⊥, τ')]>Γ ⊢ τ^x :: *@O ->
-    x ∉ fv τ ∪ dom aset Γ ∪ tctx_fv Γ ->
-    Γ ⊢ let e in τ :: *@O.
-  Proof.
-    typing_intro_solver.
-  Qed.
-
-  Lemma KProd_intro Γ τ1 τ2 κ1 κ2 :
-    Γ ⊢ τ1 :: κ1 ->
-    Γ ⊢ τ2 :: κ2 ->
-    Γ ⊢ τ1 * τ2 :: (κ1 ⊔ κ2).
-  Proof.
-    eauto using kinding, join_ub_l, join_ub_r.
-  Qed.
-
-End typing_kinding_intro.
+End admissible.
 
 (** * Tactics *)
 
@@ -339,47 +326,47 @@ blindly. *)
 constructors. *)
 Ltac typing_intro_ :=
   lazymatch goal with
-  | |- _; _ ⊢ fvar _ : _ => eapply TFVar
-  | |- _; _ ⊢ gvar _ : _ => eapply TGVar
-  | |- _; _ ⊢ \:{_}_ => _ : _ => eapply TAbs_intro
-  | |- _; _ ⊢ let _ in _ : _ => eapply TLet_intro
-  | |- _; _ ⊢ _ _ : _ => eapply TApp
-  | |- _; _ ⊢ () : _ => eapply TUnit
-  | |- _; _ ⊢ lit _ : _ => eapply TLit
-  | |- _; _ ⊢ s𝔹 _ : _ => eapply TSec
-  | |- _; _ ⊢ (_, _) : _ => eapply TPair
-  | |- _; _ ⊢ ~if _ then _ else _ : _ => eapply TOIte
-  | |- _; _ ⊢ π@_ _ : _ => eapply TProj
-  | |- _; _ ⊢ inj@_<_> _ : _ => eapply TInj
-  | |- _; _ ⊢ ~inj@_<_> _ : _ => eapply TOInj
-  | |- _; _ ⊢ ~case _ of _ | _ : _ => eapply TOCase_intro
-  | |- _; _ ⊢ fold<_> _ : _ => eapply TFold
-  | |- _; _ ⊢ unfold<_> _ : _ => eapply TUnfold
-  | H : _; _ ⊢ ?e :{⊥} _ |- _; _ ⊢ if ?e then _ else _ : _ => eapply TIte
-  | |- _; _ ⊢ if _ then _ else _ : _ => eapply TIteNoDep
-  | H : _; _ ⊢ ?e :{⊥} _ |- _; _ ⊢ case ?e of _ | _ : _ => eapply TCase_intro
-  | |- _; _ ⊢ case _ of _ | _ : _ => eapply TCaseNoDep_intro
-  | |- _; _ ⊢ tape _ : _ => eapply TTape
-  | |- _; _ ⊢ mux _ _ _ : _ => eapply TMux
-  | |- _; _ ⊢ [_] : _ => eapply TBoxedLit
-  | |- _; _ ⊢ [inj@_<_> _] : _ => eapply TBoxedInj
-  | |- _; _ ⊢ ?e : ?τ => is_var e; assert_fails (is_evar τ); eapply TConv
+  | |- _ ⊢ fvar _ : _ => eapply TFVar
+  | |- _ ⊢ gvar _ : _ => eapply TGVar
+  | |- _ ⊢ \:{_}_ => _ : _ => eapply TAbs_intro
+  | |- _ ⊢ let _ in _ : _ => eapply TLet_intro
+  | |- _ ⊢ _ _ : _ => eapply TApp
+  | |- _ ⊢ () : _ => eapply TUnit
+  | |- _ ⊢ lit _ : _ => eapply TLit
+  | |- _ ⊢ s𝔹 _ : _ => eapply TSec
+  | |- _ ⊢ (_, _) : _ => eapply TPair
+  | |- _ ⊢ ~if _ then _ else _ : _ => eapply TOIte
+  | |- _ ⊢ π@_ _ : _ => eapply TProj
+  | |- _ ⊢ inj@_<_> _ : _ => eapply TInj
+  | |- _ ⊢ ~inj@_<_> _ : _ => eapply TOInj
+  | |- _ ⊢ ~case _ of _ | _ : _ => eapply TOCase_intro
+  | |- _ ⊢ fold<_> _ : _ => eapply TFold
+  | |- _ ⊢ unfold<_> _ : _ => eapply TUnfold
+  | H : _ ⊢ ?e :{⊥} _ |- _; _ ⊢ if ?e then _ else _ : _ => eapply TIte
+  | |- _ ⊢ if _ then _ else _ : _ => eapply TIteNoDep
+  | H : _ ⊢ ?e :{⊥} _ |- _; _ ⊢ case ?e of _ | _ : _ => eapply TCase_intro
+  | |- _ ⊢ case _ of _ | _ : _ => eapply TCaseNoDep_intro
+  | |- _ ⊢ tape _ : _ => eapply TTape
+  | |- _ ⊢ mux _ _ _ : _ => eapply TMux
+  | |- _ ⊢ [_] : _ => eapply TBoxedLit
+  | |- _ ⊢ [inj@_<_> _] : _ => eapply TBoxedInj
+  | |- _ ⊢ ?e : ?τ => is_var e; assert_fails (is_evar τ); eapply TConv
   end.
 
 Ltac kinding_intro_ :=
   lazymatch goal with
-  | |- _; _ ⊢ gvar _ :: _ => eapply KGVar
-  | |- _; _ ⊢ 𝟙 :: _ => eapply KUnit
-  | |- _; _ ⊢ 𝔹{_} :: _ => eapply KBool
-  | |- _; _ ⊢ Π:{_}_, _ :: _ => eapply KPi_intro
-  | |- _; _ ⊢ _@_ :: _ => eapply KApp
-  | |- _; _ ⊢ _ * _ :: _ => eapply KProd_intro
-  | |- _; _ ⊢ _ + _ :: _ => eapply KSum
-  | |- _; _ ⊢ _ ~+ _ :: _ => eapply KOSum
-  | |- _; _ ⊢ if _ then _ else _ :: _ => eapply KIte
-  | |- _; _ ⊢ case _ of _ | _ :: _ => eapply KCase_intro
-  | |- _; _ ⊢ let _ in _ :: _ => eapply KLet_intro
-  | |- _; _ ⊢ ?τ :: ?κ => is_var τ; assert_fails (is_evar κ); eapply KSub
+  | |- _ ⊢ gvar _ :: _ => eapply KGVar
+  | |- _ ⊢ 𝟙 :: _ => eapply KUnit
+  | |- _ ⊢ 𝔹{_} :: _ => eapply KBool
+  | |- _ ⊢ Π:{_}_, _ :: _ => eapply KPi_intro
+  | |- _ ⊢ _@_ :: _ => eapply KApp
+  | |- _ ⊢ _ * _ :: _ => eapply KProd_intro
+  | |- _ ⊢ _ + _ :: _ => eapply KSum
+  | |- _ ⊢ _ ~+ _ :: _ => eapply KOSum
+  | |- _ ⊢ if _ then _ else _ :: _ => eapply KIte
+  | |- _ ⊢ case _ of _ | _ :: _ => eapply KCase_intro
+  | |- _ ⊢ let _ in _ :: _ => eapply KLet_intro
+  | |- _ ⊢ ?τ :: ?κ => is_var τ; assert_fails (is_evar κ); eapply KSub
   end.
 
 Tactic Notation "typing_kinding_intro_" tactic3(tac) :=
@@ -399,6 +386,6 @@ Ltac kinding_intro :=
 
 Ltac typing_kinding_intro :=
   lazymatch goal with
-  | |- _; _ ⊢ _ : _ => typing_intro
-  | |- _; _ ⊢ _ :: _ => kinding_intro
+  | |- _ ⊢ _ : _ => typing_intro
+  | |- _ ⊢ _ :: _ => kinding_intro
   end.
