theories/lang_oadt/weakening.v
@@ -1,0 +1,96 @@
+From oadt Require Import lang_oadt.base.
+From oadt Require Import lang_oadt.syntax.
+From oadt Require Import lang_oadt.semantics.
+From oadt Require Import lang_oadt.typing.
+
+Import syntax.notations.
+Import typing.notations.
+
+(** * Weakening lemmas  *)
+
+Lemma pared_weakening Σ e e' :
+  Σ ⊢ e ⇛ e' ->
+  forall Σ', Σ ⊆ Σ' ->
+        Σ' ⊢ e ⇛ e'.
+Proof.
+  induction 1; intros;
+    econstructor; eauto using lookup_weaken.
+Qed.
+
+Lemma pared_equiv_weakening Σ e e' :
+  Σ ⊢ e ≡ e' ->
+  forall Σ', Σ ⊆ Σ' ->
+        Σ' ⊢ e ≡ e'.
+Proof.
+  induction 1; intros; qauto use: pared_equiv, pared_weakening.
+Qed.
+
+Lemma weakening_ Σ :
+  (forall Γ e l τ,
+    Σ; Γ ⊢ e :{l} τ ->
+    forall Σ' Γ',
+      Σ ⊆ Σ' ->
+      Γ ⊆ Γ' ->
+      Σ'; Γ' ⊢ e :{l} τ) /\
+  (forall Γ τ κ,
+    Σ; Γ ⊢ τ :: κ ->
+    forall Σ' Γ',
+      Σ ⊆ Σ' ->
+      Γ ⊆ Γ' ->
+      Σ'; Γ' ⊢ τ :: κ).
+Proof.
+  apply typing_kinding_mutind; intros; subst;
+    try qauto l: on ctrs: typing, kinding;
+    try qauto l: on use: lookup_weaken ctrs: typing, kinding;
+    try qauto l: on use: insert_mono ctrs: typing, kinding;
+    (* For the [case]/[~case] cases and the [TConv] case. *)
+    econstructor; eauto using insert_mono; qauto use: pared_equiv_weakening.
+Qed.
+
+Lemma weakening Σ Γ Σ' Γ' e l τ :
+  Σ; Γ ⊢ e :{l} τ ->
+  Σ ⊆ Σ' ->
+  Γ ⊆ Γ' ->
+  Σ'; Γ' ⊢ e :{l} τ.
+Proof.
+  hauto use: weakening_.
+Qed.
+
+Lemma kinding_weakening Σ Γ Σ' Γ' τ κ :
+  Σ; Γ ⊢ τ :: κ ->
+  Σ ⊆ Σ' ->
+  Γ ⊆ Γ' ->
+  Σ'; Γ' ⊢ τ :: κ.
+Proof.
+  hauto use: weakening_.
+Qed.
+
+Lemma weakening_empty Σ Γ e l τ :
+  Σ; ∅ ⊢ e :{l} τ ->
+  Σ; Γ ⊢ e :{l} τ.
+Proof.
+  eauto using weakening, map_empty_subseteq.
+Qed.
+
+Lemma kinding_weakening_empty Σ Γ τ κ :
+  Σ; ∅ ⊢ τ :: κ ->
+  Σ; Γ ⊢ τ :: κ.
+Proof.
+  eauto using kinding_weakening, map_empty_subseteq.
+Qed.
+
+Lemma weakening_insert Σ Γ e l τ τ' x :
+  Σ; Γ ⊢ e :{l} τ ->
+  x ∉ dom aset Γ ->
+  Σ; (<[x:=τ']>Γ) ⊢ e :{l} τ.
+Proof.
+  eauto using weakening, insert_fresh_subseteq.
+Qed.
+
+Lemma kinding_weakening_insert Σ Γ τ τ' κ x :
+  Σ; Γ ⊢ τ :: κ ->
+  x ∉ dom aset Γ ->
+  Σ; (<[x:=τ']>Γ) ⊢ τ :: κ.
+Proof.
+  eauto using kinding_weakening, insert_fresh_subseteq.
+Qed.
